Slight clean up

src/rocq/Theory/I2F/I2F_interp.v
@@ -1,10 +1,13 @@
+(** * I2F invariant for the handlers *)
+
 From Equations Require Import Equations.
 
 From Stdlib Require Import
   ZArith
   Strings.String
   List
-  Morphisms.
+  Morphisms
+  Equality.
 Import ListNotations.
 
 From ITree Require Import Basics.HeterogeneousRelations ITree InterpFacts Eq.
@@ -33,19 +36,18 @@ From Vellvm Require Import
 From Vellvm Require Import
   Theory.I2F.Refinement
   Theory.I2F.I2F_exp
-  Theory.I2F.I2F_MemS.
+  Theory.I2F.I2F_MemS
+  Theory.I2F.I2F_memory.
 
 Existing Instance MemoryModelStateV.
 Existing Instance MemoryModelPrimitivesV.
 
+Import Monads State StateFacts.
 From Paco Require Import paco.
 
-(** ** [pure_base_to_semantic]-wrapped intrinsics
+(** * Intrinsics (out of the memory model) *)
 
-    [pure_base_to_semantic f := pure_to_semantic (pure_base_to_pure f)],
-    [pure_to_semantic f args _ := EOU_to_itree (f args)]: a purely EOU-level
-    computation over base values, lifted to [semantic_function]. Reduces via
-    [I2F_refine_lift] to an [I2F_EOU] fact about [pure_base_to_pure]. *)
+(** ** [pure_base_to_semantic]-wrapped intrinsics *)
 
 Lemma I2F_pure_base_to_semantic :
   forall (f1 : @pure_base_function PInf) (f2 : @pure_base_function PFin),
@@ -68,10 +70,7 @@ Proof.
   destruct Hans; apply I2F_EOU_ret; constructor; constructor; auto.
 Qed.
 
-(** ** The 11 leaf [pure_base_function]s: none of these touch [DVALUE_Pointer]
-    or [DVALUE_Iptr], so wherever the pattern actually matches,
-    [I2F_dvalue_base]'s Float/Double/Int constructors force the two sides to
-    carry the *same* payload. *)
+(** ** The 11 leaf [pure_base_function]s: none of these touch [DVALUE_Pointer] or [DVALUE_Iptr] *)
 
 Lemma I2F_llvm_fabs_f32 : forall args1 args2,
     Forall2 I2F_dvalue_base args1 args2 ->
@@ -335,7 +334,292 @@ Proof.
     simp I2FA_Intrinsic in Hab.
     simp I2FA_Intrinsic.
 Qed.
-  
+
+
+(** * Relating [FusedS], the product state threaded by [interp_mcfg] *)
+
+(** ** [local_env] / [global_env] *)
+
+Definition I2F_env : @local_env PInf -> @local_env PFin -> Prop := RM_Refine I2F_dvalue.
+Definition I2F_local_env : @local_env PInf -> @local_env PFin -> Prop := I2F_env.
+Definition I2F_global_env : @global_env PInf -> @global_env PFin -> Prop := I2F_env.
+
+(** ** [stack_frame] / [stack] *)
+
+Record I2F_stack_frame (f1 : @stack_frame PInf) (f2 : @stack_frame PFin) : Prop :=
+  { i2f_sf_vars : I2F_local_env f1.(stack_vars) f2.(stack_vars);
+    i2f_sf_exc  : option_rel I2F_dvalue f1.(stack_exc) f2.(stack_exc);
+    i2f_sf_loc  : f1.(stack_loc) = f2.(stack_loc);
+  }.
+
+Definition I2F_stack : @stack PInf -> @stack PFin -> Prop := Forall2 I2F_stack_frame.
+
+(** ** [FusedS] itself *)
+
+Record I2F_FusedS (s1 : @FusedS PInf) (s2 : @FusedS PFin) : Prop :=
+  { i2f_fs_mem   : I2F_State (fst s1) (fst s2);
+    i2f_fs_frame : I2F_stack_frame (fst (fst (snd s1))) (fst (fst (snd s2)));
+    i2f_fs_stack : I2F_stack (snd (fst (snd s1))) (snd (fst (snd s2)));
+    i2f_fs_genv  : I2F_global_env (snd (snd s1)) (snd (snd s2));
+  }.
+
+(** * Per-handler compatibility *)
+
+(** * Globals *)
+Lemma I2F_fused_global :
+  forall T1 T2 (e1 : @GlobalE PInf T1) (e2 : @GlobalE PFin T2),
+    I2FE_Global e1 e2 ->
+    forall s1 s2, I2F_FusedS s1 s2 ->
+      I2F_refine_MCFGbot
+        (prod_rel I2F_FusedS (fun r1 r2 => I2FA_Global e1 r1 e2 r2))
+        (fused_global e1 s1) (fused_global e2 s2).
+Proof.
+  intros T1 T2 e1 e2 H [m1 [ls1 g1]] [m2 [ls2 g2]] Hs.
+  destruct Hs as [Hmem Hframe Hstack Hgenv]; cbn in Hmem, Hframe, Hstack, Hgenv.
+  destruct e1 as [x1 dv1 | x1]; destruct e2 as [x2 dv2 | x2];
+    simp I2FE_Global in H; cbn in H; try contradiction.
+  - (* GlobalWrite *)
+    destruct H as [-> Hdv].
+    unfold fused_global, on_genv, handle_global_debug, handle_global, update_globals_ref,
+      I2F_refine_MCFGbot; cbn; rewrite ?Eqit.bind_ret_l.
+    apply ruttc_ret.
+    split.
+    + constructor; cbn; auto.
+      apply RM_Refine_add; auto.
+    + simp I2FA_Global; auto.
+  - (* GlobalRead *)
+    subst.
+    unfold fused_global, on_genv, handle_global_debug, handle_global, update_globals_ref,
+      I2F_refine_MCFGbot; cbn.
+    pose proof (RM_Refine_lookup I2F_dvalue g1 g2 Hgenv x2) as Hlk.
+    unfold rid_lookup in Hlk.
+    destruct Hlk as [ | dv1 dv2 Hdv]; cbn; rewrite ?Eqit.bind_ret_l.
+    + rbind (fun _ _ => False);
+        [rbind (fun _ _ => False);
+          [apply ruttc_trigger_cast; cbnn; first [simp I2FE_Failure | simp I2FE_UB]; auto |
+            intros _ _ []] |
+          intros _ _ []].
+    + apply ruttc_ret. split; [constructor; cbn; auto | simp I2FA_Global; auto].
+Qed.
+
+(** * Locals *)
+Lemma I2F_fused_local :
+  forall T1 T2 (e1 : @LocalE PInf T1) (e2 : @LocalE PFin T2),
+    I2FE_Local e1 e2 ->
+    forall s1 s2, I2F_FusedS s1 s2 ->
+      I2F_refine_MCFGbot
+        (prod_rel I2F_FusedS (fun r1 r2 => I2FA_Local e1 r1 e2 r2))
+        (fused_local e1 s1) (fused_local e2 s2).
+Proof.
+  intros T1 T2 e1 e2 H [m1 [[f1 stk1] g1]] [m2 [[f2 stk2] g2]] Hs.
+  destruct Hs as [Hmem Hframe Hstack Hgenv]; cbn in Hmem, Hframe, Hstack, Hgenv.
+  destruct Hframe as [Hvars Hexc Hloc]; cbn in Hvars, Hexc, Hloc.
+  destruct e1 as [x1 dv1 | x1]; destruct e2 as [x2 dv2 | x2];
+    simp I2FE_Local in H; cbn in H; try contradiction.
+  - (* LocalWrite *)
+    destruct H as [-> Hdv].
+    unfold fused_local, on_ls, handle_local_stack, handle_local_debug, handle_local,
+      update_locals_ref, upd_local_sf, I2F_refine_MCFGbot; cbn; rewrite ?Eqit.bind_ret_l.
+    apply ruttc_ret.
+    split.
+    + constructor; cbn; auto.
+      constructor; cbn; auto.
+      apply RM_Refine_add; auto.
+    + simp I2FA_Local; auto.
+  - (* LocalRead *)
+    subst.
+    unfold fused_local, on_ls, handle_local_stack, handle_local_debug, handle_local,
+      update_locals_ref, I2F_refine_MCFGbot; cbn.
+    pose proof (RM_Refine_lookup I2F_dvalue (stack_vars f1) (stack_vars f2) Hvars x2) as Hlk.
+    unfold rid_lookup in Hlk.
+    destruct Hlk as [ | dv1 dv2 Hdv]; cbn; rewrite ?Eqit.bind_ret_l.
+    + rbind (fun _ _ => False);
+        [rbind (fun _ _ => False);
+          [rbind (fun _ _ => False);
+            [apply ruttc_trigger_cast; cbnn; first [simp I2FE_Failure | simp I2FE_UB]; auto |
+              intros _ _ []] |
+            intros _ _ []] |
+          intros _ _ []].
+    + apply ruttc_ret.
+      split; [constructor; cbn; auto; constructor; cbn; auto | simp I2FA_Local; auto].
+Qed.
+
+(** * Stack *)
+Lemma I2F_fused_stack :
+  forall T1 T2 (e1 : @StackE PInf T1) (e2 : @StackE PFin T2),
+    I2FE_Stack e1 e2 ->
+    forall s1 s2, I2F_FusedS s1 s2 ->
+      I2F_refine_MCFGbot
+               (prod_rel I2F_FusedS (fun r1 r2 => I2FA_Stack e1 r1 e2 r2))
+        (fused_stack e1 s1) (fused_stack e2 s2).
+Proof.
+  intros T1 T2 e1 e2 H [m1 [[f1 stk1] g1]] [m2 [[f2 stk2] g2]] Hs.
+  destruct Hs as [Hmem Hframe Hstack Hgenv]; cbn in Hmem, Hframe, Hstack, Hgenv.
+  destruct e1 as [args1 | |exc1| ]; destruct e2 as [args2 | |exc2| ];
+    simp I2FE_Stack in H; cbn in H; try contradiction.
+  - (* StackPush *)
+    unfold fused_stack, on_ls, handle_stack, I2F_refine_MCFGbot; cbn; rewrite ?Eqit.bind_ret_l.
+    assert (Hinit : I2F_local_env
+                      (fold_right (fun '(x,dv) => Maps.add x dv) Maps.empty args1)
+                      (fold_right (fun '(x,dv) => Maps.add x dv) Maps.empty args2)).
+    { induction H as [ | [x1 dv1] [x2 dv2] l1 l2 Hxd Hrest IH]; cbn.
+      - apply RM_Refine_empty.
+      - destruct Hxd as [Heq Hdv]; cbn in Heq; subst.
+        apply RM_Refine_add; auto. }
+    apply ruttc_ret.
+    split.
+    + constructor; cbn.
+      * auto.
+      * constructor; cbn; [auto | constructor | auto].
+      * constructor; auto.
+      * auto.
+    + simp I2FA_Stack; auto.
+  - (* StackPop *)
+    unfold fused_stack, on_ls, handle_stack, I2F_refine_MCFGbot; cbn.
+    destruct Hstack as [ | f1' f2' stk1' stk2' Hf' Hstk'].
+    + cbn; rewrite ?Eqit.bind_ret_l.
+      rbind (fun _ _ => False);
+        [rbind (fun _ _ => False);
+          [apply ruttc_trigger;
+            [cbnn; first [simp I2FE_Failure | simp I2FE_UB]; auto | intros [] [] _] |
+            intros _ _ []] |
+          intros _ _ []].
+    + cbn; rewrite ?Eqit.bind_ret_l.
+      apply ruttc_ret.
+      split; [constructor; cbn; auto | simp I2FA_Stack; auto].
+  - (* StackRaise *)
+    unfold fused_stack, on_ls, handle_stack, I2F_refine_MCFGbot; cbn; rewrite ?Eqit.bind_ret_l.
+    apply ruttc_ret.
+    destruct Hframe as [Hvars Hexc Hloc].
+    split.
+    + constructor; cbn.
+      * auto.
+      * constructor; cbn; [auto | constructor; auto | auto].
+      * auto.
+      * auto.
+    + simp I2FA_Stack; auto.
+  - (* StackGetExc *)
+    unfold fused_stack, on_ls, handle_stack, I2F_refine_MCFGbot; cbn; rewrite ?Eqit.bind_ret_l.
+    apply ruttc_ret.
+    destruct Hframe as [Hvars Hexc Hloc].
+    split.
+    + constructor; cbn.
+      * auto.
+      * constructor; cbn; [auto | constructor | auto].
+      * auto.
+      * auto.
+    + simp I2FA_Stack; auto.
+Qed.
+
+(** * Memory
+Note: This essentially lifts [I2F_handle_memoryM], but through the monad morphism implementing
+[memM] in a deterministic way. This is the main piece of proof that will have to be
+adapted for the model. *)
+
+(** [fresh_provenance] resolves via [next_provenance] *)
+Lemma I2F_fresh_provenance_eq :
+  forall s1 s2,
+    I2F_State s1 s2 ->
+    next_provenance (state_provenance s1) = next_provenance (state_provenance s2).
+Proof.
+  intros s1 s2 [_ Hprov]; cbn in *; rewrite Hprov; reflexivity.
+Qed.
+
+(** ** Interpreter-specific: [memM_interp] *)
+Lemma I2F_memM_interp R1 R2 RR (t1 : @memM PInf _ R1) (t2 : @memM PFin _ R2) :
+  I2F_memS I2F_State RR t1 t2 ->
+  forall s1 s2,
+    I2F_State s1 s2 ->
+    I2F_refine_MCFGbot (prod_rel I2F_State RR) (memM_interp t1 s1) (memM_interp t2 s2).
+Proof.
+  induction 1 as [x1 x2 Hr | e1 e2 | e m2 | m1 e
+                  | k1 k2 Hget IHget | σ1 σ2 k1 k2 Hσ Hput IHput
+                  | c k1 k2 Hc IHc];
+    intros s1 s2 HS; cbn.
+  - pstep; constructor; constructor; auto.
+  - apply ruttc_trigger_cast; constructor.
+  - unfold raiseUB, trigger_cast; rewrite bind_trigger.
+    pstep; repeat constructor.
+  - unfold raiseOOM, trigger_cast; rewrite bind_trigger.
+    pstep; repeat constructor.
+  - now apply IHget.
+  - now apply IHput.
+  - destruct c; cbn.
+    + (* Cnext_key *)
+      pose proof (I2F_next_key_with_alignment
+                    (i2f_ms_memory (i2f_st_ms HS)) align) as Heq.
+      rewrite Heq.
+      apply IHc; auto.
+    + (* Cfresh_prov *)
+      rewrite !Eqit.bind_ret_l.
+      pose proof (I2F_fresh_provenance_eq HS) as Heq.
+      cbn in Heq.
+      rewrite Heq.
+      apply IHc.
+      constructor; cbn; [exact (i2f_st_ms HS) | reflexivity].
+    + (* Cexposed_prov *)
+      now apply IHc.
+Qed.
+
+Lemma I2F_fused_memory :
+  forall T1 T2 (e1 : @MemoryE PInf T1) (e2 : @MemoryE PFin T2),
+    I2FE_Memory e1 e2 ->
+    forall s1 s2, I2F_FusedS s1 s2 ->
+             I2F_refine_MCFGbot
+               (prod_rel I2F_FusedS (fun r1 r2 => I2FA_Memory e1 r1 e2 r2))
+               (fused_memory e1 s1) (fused_memory e2 s2).
+Proof.
+  intros * HM * HS.
+  unfold fused_memory.
+  unfold handle_memory.
+  destruct s1,s2,HS; cbn in *.
+  cbn in *.
+  eapply ruttc_bind.
+  apply I2F_memM_interp; [apply I2F_handle_memoryM; auto |]; auto.
+  intros [] [] []; pstep; do 2 constructor; cbn; auto.
+  constructor; auto.
+Qed.
+
+(** * Intrinsics (the internal to the memory-model ones) *)
+(* TODO: Define this lifting of Answer relations to value ones given two events *)
+Lemma I2F_fused_intrinsic :
+  forall T1 T2 (e1 : @IntrinsicE PInf T1) (e2 : @IntrinsicE PFin T2),
+    I2FE_Intrinsic e1 e2 ->
+    forall s1 s2, I2F_FusedS s1 s2 ->
+      I2F_refine_MCFGbot
+        (prod_rel I2F_FusedS (fun r1 r2 => I2FA_Intrinsic e1 r1 e2 r2))
+        (fused_intrinsic e1 s1) (fused_intrinsic e2 s2).
+Proof.
+  intros * HI * HS.
+  unfold fused_intrinsic.
+  unfold handle_intrinsic.
+  destruct s1,s2,HS; cbn in *.
+  cbn.
+  eapply ruttc_bind.
+  apply I2F_memM_interp; [apply I2F_handle_intrinsicM; auto |]; auto.
+  intros [] [] []; pstep; do 2 constructor; cbn; auto.
+  constructor; auto.
+Qed.
+
+(** * Draw *)
+Lemma I2F_fused_draw :
+  forall T1 T2 (e1 : @DrawE PInf T1) (e2 : @DrawE PFin T2),
+    I2FE_Draw e1 e2 ->
+    forall s1 s2, I2F_FusedS s1 s2 ->
+      I2F_refine_MCFGbot
+        (prod_rel I2F_FusedS (fun r1 r2 => I2FA_Draw e1 r1 e2 r2))
+        (fused_draw e1 s1) (fused_draw e2 s2).
+Proof.
+  intros T1 T2 e1 e2 H s1 s2 Hs.
+  destruct e1 as [τ1]; destruct e2 as [τ2].
+  simp I2FE_Draw in H; subst.
+  unfold fused_draw, handle_draw, I2F_refine_MCFGbot.
+  erbind; [apply I2F_refine_lift_bot, I2F_default_dvalue_of_dtyp |].
+  intros r1 r2 Hr; apply ruttc_ret; auto.
+Qed.
+
+
+(** * Lifting the intrinsic handler to [interp_intrinsics] *)
 Lemma I2F_interp_intrinsics {R1 R2} (RR : R1 -> R2 -> Prop)
   (t1 : @MCFGtop PInf R1) (t2 : @MCFGtop PFin R2):
   I2F_refine_MCFG RR t1 t2 ->
@@ -355,5 +639,175 @@ Proof.
     destruct e1 as [e1|e1]; destruct e2 as [e2|e2]; try elim HEv.
     2:apply ruttc_trigger; auto.
     now apply I2F_handle_intrinsics.
+Qed.
+
+(** * Assembling the six per-handler lemmas into [interp_vellvm_h] *)
+Lemma I2F_interp_vellvm_h :
+  forall T1 T2 (e1 : @MCFGEtop PInf T1) (e2 : @MCFGEtop PFin T2),
+    I2FE_MCFG e1 e2 ->
+    forall s1 s2, I2F_FusedS s1 s2 ->
+      I2F_refine_MCFGbot
+        (prod_rel I2F_FusedS (fun r1 r2 => I2FA_MCFG e1 r1 e2 r2))
+        (interp_vellvm_h e1 s1) (interp_vellvm_h e2 s2).
+Proof.
+  intros T1 T2 e1 e2 H s1 s2 Hs.
+  unfold interp_vellvm_h.
+  destruct e1 as [e1|e1]; destruct e2 as [e2|e2]; cbn in H; cbn; try easy.
+  { (* ExternalCallE *)
+    unfold fused_trigger.
+    destruct e1 as [t1 f1 args1 | str1 | str1]; destruct e2 as [t2 f2 args2 | str2 | str2];
+      simp I2FE_ExternalCall in H; cbn in H; try contradiction.
+    - (* ExternalCall *)
+      rbind I2F_dvalue.
+      apply ruttc_trigger;
+      [cbnn; simp I2FE_ExternalCall; auto |
+      intros a b Hab; cbnn in Hab; simp I2FA_ExternalCall in Hab].
+      intros r1 r2 Hr; rstep.
+    - (* IO_stdout *)
+      rbind Logic.eq.
+      apply ruttc_trigger;
+      [cbnn; simp I2FE_ExternalCall; auto |
+      intros [] [] Hab; cbnn in Hab; simp I2FA_ExternalCall in Hab;
+                  simp I2FA_ExternalCall; auto].
+      intros r1 r2 <-; rstep.
+      constructor; auto.
+      cbn; simp I2FA_ExternalCall; auto.
+    - (* IO_stderr *)
+      rbind Logic.eq.
+      apply ruttc_trigger;
+      [cbnn; simp I2FE_ExternalCall; auto |
+      intros [] [] Hab; cbnn in Hab; simp I2FA_ExternalCall in Hab;
+      simp I2FA_ExternalCall; auto].
+      intros r1 r2 <-; rstep.
+      constructor; auto.
+      cbn; simp I2FA_ExternalCall; auto.
+  }
+  destruct e1 as [e1|e1]; destruct e2 as [e2|e2]; cbn in H; cbn; try easy;
+    [apply I2F_fused_intrinsic; auto |].
+  destruct e1 as [e1|e1]; destruct e2 as [e2|e2]; cbn in H; cbn; try easy;
+    [apply I2F_fused_global; auto|].
+  destruct e1 as [e1|e1]; destruct e2 as [e2|e2]; cbn in H; cbn; try easy.
+  destruct e1 as [e1|e1]; destruct e2 as [e2|e2]; cbn in H; cbn; try easy;
+    [apply I2F_fused_local; auto | apply I2F_fused_stack; auto].
+  destruct e1 as [e1|e1]; destruct e2 as [e2|e2]; cbn in H; cbn; try easy;
+    [apply I2F_fused_memory; auto|].
+  destruct e1 as [e1|e1]; destruct e2 as [e2|e2]; cbn in H; cbn; try easy;
+    [apply I2F_fused_draw; auto|].
+  destruct e1 as [e1|e1]; destruct e2 as [e2|e2]; cbn in H; cbn; try easy;
+  [apply ruttc_trigger'; cbnn; auto |].
+  destruct e1 as [e1|e1]; destruct e2 as [e2|e2]; cbn in H; cbn; try easy;
+  [apply ruttc_trigger'; cbnn; auto |].
+  destruct e1 as [e1|e1]; destruct e2 as [e2|e2]; cbn in H; cbn; try easy;
+  [apply ruttc_trigger'; cbnn; auto |].
+  destruct e1 as [e1|e1]; destruct e2 as [e2|e2]; cbn in H; cbn; try easy;
+  [apply ruttc_trigger'; cbnn; auto |].
+  apply ruttc_trigger'; cbnn; auto.
+Qed.
+
+(** * Transporting [ruttc] through [interp_state]
+    This should be a generic lemma on [ruttc] and stateful interpreters,
+    but the statement w.r.t. changing signatures is tricky
+ *)
+Lemma ruttc_interp_state_specialized {R1 R2} (RR : R1 -> R2 -> Prop) t1 t2
+  (HR: I2F_refine_MCFG RR t1 t2):
+  forall s1 s2,
+    I2F_FusedS s1 s2 ->
+    I2F_refine_MCFGbot (prod_rel I2F_FusedS RR)
+      (interp_state interp_vellvm_h t1 s1)
+      (interp_state interp_vellvm_h t2 s2).
+Proof.
+  ginit.
+  revert t1 t2 HR.
+  gcofix cih; intros.
+  rewrite 2 unfold_interp_state.
+  punfold HR; red in HR.
+  induction HR; pclearbot.
+  - cbn; gstep; constructor; auto.
+  - cbn; gstep; constructor.
+    gfinal; left; auto.
+  - cbn.
+    (* TODO fix *)
+    guclo (@ruttc_clo_bind
+             (@MCFGEbot PInf) (@MCFGEbot PFin) (@FusedS PInf * R1) (@FusedS PFin * R2)).
+    econstructor.
+    apply I2F_interp_vellvm_h; auto.
+    intros [] [] []; cbn in *.
+    gstep; constructor.
+    gfinal; left; apply cih; auto.
+    apply H1; auto.
+  - cbn. rewrite tau_euttge.
+    rewrite unfold_interp_state.
+    apply IHHR.
+  - cbn. rewrite tau_euttge.
+    rewrite unfold_interp_state.
+    apply IHHR.
+  - cbn.
+    generalize H; intros tmp.
+    dependent induction H.
+    cbnn; rewrite Eqit.bind_bind,bind_trigger.
+    gstep; constructor; auto; constructor.
+   - cbn.
+    generalize H; intros tmp.
+    dependent induction H.
+    cbnn; rewrite Eqit.bind_bind,bind_trigger.
+    gstep; constructor; auto; constructor.
+Qed.
+
+
+(** * The main result from this file: [interp_mcfg] *)
+(* TODO: Should this be generalized to an arbitrary relation on R? *)
+Lemma I2F_interp_mcfg {R} (t1 : @MCFGtop PInf R) (t2 : @MCFGtop PFin R):
+  I2F_refine_MCFG Logic.eq t1 t2 ->
+  forall s1 s2, I2F_FusedS s1 s2 ->
+  I2F_refine_MCFGbot (prod_rel I2F_FusedS Logic.eq)
+    (interp_mcfg t1 s1)
+    (interp_mcfg t2 s2).
+Proof.
+  intros Hmcfg * Hfused.
+  apply ruttc_interp_state_specialized; auto.
+  apply I2F_interp_intrinsics; auto.
+Qed.
+
+(** * Additional utility lemmas for the top-level *)
+
+Lemma I2F_interp_mcfg_ret {R1 R2} (RR : R1 -> R2 -> Prop) (r1 : R1) (r2 : R2) :
+  RR r1 r2 ->
+  forall s1 s2, I2F_FusedS s1 s2 ->
+    I2F_refine_MCFGbot (prod_rel I2F_FusedS RR)
+      (interp_mcfg (Ret r1) s1) (interp_mcfg (Ret r2) s2).
+Proof.
+  intros Hr s1 s2 Hs.
+  unfold interp_mcfg.
+  apply ruttc_interp_state_specialized; auto.
+  apply I2F_interp_intrinsics, ruttc_ret; auto.
+Qed.
+
+Lemma I2F_interp_mcfg_bind {R1 R2 T1 T2} (RR : R1 -> R2 -> Prop) (RT : T1 -> T2 -> Prop)
+  (t1 : @MCFGtop PInf R1) (t2 : @MCFGtop PFin R2)
+  (k1 : R1 -> @MCFGtop PInf T1) (k2 : R2 -> @MCFGtop PFin T2) :
+  I2F_refine_MCFG RR t1 t2 ->
+  (forall r1 r2, RR r1 r2 -> I2F_refine_MCFG RT (k1 r1) (k2 r2)) ->
+  forall s1 s2, I2F_FusedS s1 s2 ->
+    I2F_refine_MCFGbot (prod_rel I2F_FusedS RT)
+      (interp_mcfg (ITree.bind t1 k1) s1) (interp_mcfg (ITree.bind t2 k2) s2).
+Proof.
+  intros Ht Hk s1 s2 Hs.
+  unfold interp_mcfg.
+  apply ruttc_interp_state_specialized; auto.
+  apply I2F_interp_intrinsics.
+  eapply ruttc_bind; eauto.
+Qed.
+
+Lemma I2F_interp_mcfg_trigger :
+  forall T1 T2 (e1 : @MCFGEtop PInf T1) (e2 : @MCFGEtop PFin T2),
+    I2FE_MCFG e1 e2 ->
+    forall s1 s2, I2F_FusedS s1 s2 ->
+      I2F_refine_MCFGbot (prod_rel I2F_FusedS (fun r1 r2 => I2FA_MCFG e1 r1 e2 r2))
+        (interp_mcfg (ITree.trigger e1) s1) (interp_mcfg (ITree.trigger e2) s2).
+Proof.
+  intros * HE s1 s2 Hs.
+  unfold interp_mcfg.
+  apply ruttc_interp_state_specialized; auto.
+  apply I2F_interp_intrinsics, ruttc_trigger; auto.
 Qed.
 
